Prove eutt_interp_locals

theories/MorphismsFacts.v
@@ -245,23 +245,27 @@ Proof. rewrite itree_eta, interp1_unfold, <-itree_eta. reflexivity. Qed.
 
 (** ** [interp1] is equivalent to [interp] *)
 
-Definition interp_match {E F} (f: E ~> itree F) : (E +' F) ~> itree F :=
-  fun _ ef => match ef with inl1 e => f _ e | inr1 e => Vis e (fun r => Ret r) end.
+Section interp1_is_interp.
 
-Inductive interp_inv {E F R} (f: E ~> itree F) : relation (itree' F R) :=
+Context {E F G : Type -> Type} `{F -< G} (f : E ~> itree G).
+
+Definition interp_match : (E +' F) ~> itree G :=
+  fun _ ef => match ef with inl1 e => f _ e | inr1 e => Vis (subeffect _ e) (fun r => Ret r) end.
+
+Inductive interp_inv {R} : relation (itree' G R) :=
 | _interp_inv_main t:
-    interp_inv f
-      (observe (interp (interp_match f) _ t)) (observe (interp1 f _ t))
+    interp_inv
+      (observe (interp interp_match _ t)) (observe (interp1 f _ t))
 | _interp_inv_bind u t (k: u -> _):
-    interp_inv f
-      (observe (ITree.bind t (fun x => interp (interp_match f) _ (k x))))
+    interp_inv
+      (observe (ITree.bind t (fun x => interp interp_match _ (k x))))
       (observe (ITree.bind t (fun x => interp1 f _ (k x))))
 .
 Hint Constructors interp_inv.
 
-Lemma interp_inv_main_step E F R (f: E ~> itree F) (t: itree _ R) :
-  euttF' (fun x y => interp_inv f (observe x) (observe y)) (interp_inv f)
-         (observe (interp (interp_match f) _ t)) (observe (interp1 f _ t)).
+Lemma interp_inv_main_step R (t: itree _ R) :
+  euttF' (fun x y => interp_inv (observe x) (observe y)) interp_inv
+         (observe (interp interp_match _ t)) (observe (interp1 f _ t)).
 Proof.
   rewrite interp_unfold, interp1_unfold.
   genobs t ot. clear Heqot t.
@@ -272,11 +276,11 @@ Proof.
   fold_bind. rewrite unfold_bind. simpl. eauto.
 Qed.
 
-Lemma interp_is_interp1 E F R (f: E ~> itree F) (t: itree _ R) :
-  interp (interp_match f) _ t ≈ interp1 f _ t.
+Lemma interp_is_interp1 R (t: itree _ R) :
+  interp interp_match _ t ≈ interp1 f _ t.
 Proof.
   revert t.
-  cut (forall (t1 t2: itree _ R) (REL: interp_inv f (observe t1) (observe t2)), t1 ≈ t2).
+  cut (forall (t1 t2: itree _ R) (REL: interp_inv (observe t1) (observe t2)), t1 ≈ t2).
   { eauto. }
 
   intros. apply eutt_is_eutt'.
@@ -293,6 +297,8 @@ Proof.
     eapply upaco2_mon; eauto. intros.
     eapply (CIH' (go x2) (go x3)); eauto.
 Qed.
+
+End interp1_is_interp.
 
 Lemma eq_itree_interp1_ {E F R} (h1 h2 : E ~> itree F) :
   (forall T (e : E T), h1 _ e ≅ h2 _ e) ->
@@ -315,7 +321,7 @@ Proof.
     + intros; pupto2_final; eauto.
 Qed.
 
-Instance eq_itree_interp1 {E F R} (h : E ~> itree F) :
+Instance eq_itree_interp1 {E F G} `{F -< G} {R} (h : E ~> itree F) :
   Proper (@eq_itree (E +' F) _ _ eq ==> eq_itree eq) (interp1 h R).
 Proof.
   repeat intro.
@@ -323,8 +329,8 @@ Proof.
   reflexivity.
 Qed.
 
-Instance eutt_interp1 {E F: Type -> Type} (h: E ~> itree F) R:
-  Proper (eutt eq ==> eutt eq) (@interp1 E F F _ h R).
+Instance eutt_interp1 {E F G: Type -> Type} `{F -< G} (h: E ~> itree G) R:
+  Proper (eutt eq ==> eutt eq) (@interp1 E F G _ h R).
 Proof.
   repeat intro.
   rewrite <- 2 interp_is_interp1.
@@ -757,4 +763,16 @@ Proof.
   rewrite interp1_unfold.
   rewrite TranslateFacts.unfold_translate.
   destruct (observe t); cbn; auto.
+Qed.
+
+Lemma interp1_liftE {E F G: Type -> Type} `{F -< G}:
+  forall (h: forall T: Type, E T -> itree G T) T (e : E T),
+    @interp1 E F G _ h T (lift e) ≈ h T e.
+Proof.
+  intros. unfold lift.
+  rewrite unfold_interp1; cbn.
+  rewrite tau_eutt.
+  setoid_rewrite unfold_interp1; cbn.
+  rewrite bind_ret.
+  reflexivity.
 Qed.
